@prefix : <http://vocabularies.bridgedb.org/ops##> .
@prefix owl: <http://www.w3.org/2002/07/owl#> .
@prefix rdf: <http://www.w3.org/1999/02/22-rdf-syntax-ns#> .
@prefix xml: <http://www.w3.org/XML/1998/namespace> .
@prefix xsd: <http://www.w3.org/2001/XMLSchema#> .
@prefix rdfs: <http://www.w3.org/2000/01/rdf-schema#> .
@prefix void: <http://rdfs.org/ns/void#> .
@base <http://vocabularies.bridgedb.org/ops#> .

<http://vocabularies.bridgedb.org/ops#> rdf:type owl:Ontology ;
                                        
                                        owl:versionIRI <http://vocabularies.bridgedb.org/ops#0.120150727> ;
                                        
                                        rdfs:seeAlso <http://www.openphacts.org/specs/2013/WD-datadesc-20130912/#bridgedb> .


#################################################################
#
#    Object Properties
#
#################################################################


###  http://vocabularies.bridgedb.org/ops#assertionMethod

<http://vocabularies.bridgedb.org/ops#assertionMethod> rdf:type owl:ObjectProperty ;
                                                       
                                                       rdfs:comment "The method by which the links in the Linkset have been asserted." ;
                                                       
                                                       rdfs:domain void:Linkset ;
                                                       
                                                       rdfs:seeAlso <http://www.w3.org/TR/void/#linkset> .



###  http://vocabularies.bridgedb.org/ops#linksetJustification

<http://vocabularies.bridgedb.org/ops#linksetJustification> rdf:type owl:ObjectProperty ;
                                                            
                                                            rdfs:comment "The reason why the Linkset claims these concepts are equivalent." ;
                                                            
                                                            rdfs:domain void:Linkset .



###  http://vocabularies.bridgedb.org/ops#objectsDatatype

<http://vocabularies.bridgedb.org/ops#objectsDatatype> rdf:type owl:ObjectProperty ;
                                                       
                                                       rdfs:comment "The type of concept the objects of the triples in the Linkset represent."@en ;
                                                       
                                                       rdfs:domain void:Linkset .



###  http://vocabularies.bridgedb.org/ops#objectsSpecies

<http://vocabularies.bridgedb.org/ops#objectsSpecies> rdf:type owl:ObjectProperty ;
                                                      
                                                      rdfs:comment "The species of the concept the objects of the triples in the Linkset represent."@en ;
                                                      
                                                      rdfs:domain void:Linkset .



###  http://vocabularies.bridgedb.org/ops#subjectsDatatype

<http://vocabularies.bridgedb.org/ops#subjectsDatatype> rdf:type owl:ObjectProperty ;
                                                        
                                                        rdfs:comment "The type of concept the subjects of the triples in the Linkset represent."@en ;
                                                        
                                                        rdfs:domain void:Linkset .



###  http://vocabularies.bridgedb.org/ops#subjectsSpecies

<http://vocabularies.bridgedb.org/ops#subjectsSpecies> rdf:type owl:ObjectProperty ;
                                                       
                                                       rdfs:comment "The species of the concept the subjects of the triples in the Linkset represent."@en ;
                                                       
                                                       rdfs:domain void:Linkset .





#################################################################
#
#    Classes
#
#################################################################


###  http://rdfs.org/ns/void#Linkset

void:Linkset rdf:type owl:Class ;
             
             rdfs:isDefinedBy void: .




###  Generated by the OWL API (version 3.5.1) http://owlapi.sourceforge.net

